StandardAlgorithms/Heap/sift_down.h
@@ -1,0 +1,23 @@
+
+#ifndef SIFT_DOWN_H_INCLUDED
+#define SIFT_DOWN_H_INCLUDED
+
+#include "Heap.acsl"
+#include "MultisetReorder.acsl"
+
+/*@
+   requires   valid:    \valid(a + (0..n-1));
+   requires   bounds:   0 <= root < n;
+   requires   hfrom:    HeapFrom(a, root + 1, n);
+
+   terminates           \true;
+   exits                \false;
+   assigns              a[0..n-1];
+
+   ensures    hfrom:    HeapFrom(a, root, n);
+   ensures    reorder:  MultisetReorder{Old,Here}(a, n);
+*/
+void sift_down(value_type* a, size_type n, size_type root);
+
+#endif /* SIFT_DOWN_H_INCLUDED */
+
